Finite Map needs to export permutation and distinct

examples/FiniteMap.v
@@ -28,7 +28,6 @@ Require Export List.
 
   (* because of the dependency of values on keys, we don't just use normal lists *)
   Definition alist_t := list (sigT A.value_t).
-  Definition pair_dec (kv1 kv2:sigT A.value_t) := A.key_eq_dec (projT1 kv1) (projT1 kv2).
 
   Definition nil_al := @nil (sigT A.value_t).
   Fixpoint remove(k:A.key_t)(l:alist_t) {struct l} : alist_t := 
@@ -37,6 +36,8 @@ Require Export List.
     | (k',, v')::l' => if A.key_eq_dec k k' then remove k l'
                           else (k',, v')::(remove k l')
     end.
+
+  Definition insert(k:A.key_t)(v:A.value_t k)(l:alist_t) := (k,, v)::(remove k l).
 
   Definition coerce(k1 k2:A.key_t)(H:k1 = k2)(v:A.value_t k1) : A.value_t k2.
     intros. rewrite H in v. apply v.
@@ -51,6 +52,69 @@ Require Export List.
       | right k_neq_k' => lookup k l'
       end
     end.
+
+    Fixpoint distinct (l:alist_t) : Prop :=
+      match l with
+        | nil => True
+        | (k,,v)::ls => lookup k ls = None /\ distinct ls
+      end.
+    
+    Ltac simpler :=
+      repeat (progress ((repeat 
+        match goal with
+        | [|- context [match A.key_eq_dec ?k1 ?k2 with 
+                         | left _ => _ 
+                         | right _ => _ end]] =>
+        case_eq (A.key_eq_dec k1 k2) ; intros; try congruence ; try solve [assert False; intuition]; try subst 
+        | [H:context [match A.key_eq_dec ?k1 ?k2 with 
+                         | left _ => _ 
+                         | right _ => _ end] |- _] =>
+        destruct (A.key_eq_dec k1 k2) ; try congruence ; try solve [assert False; intuition]; try subst
+        |[H: sigT _ |- _] => destruct H
+      end); simpl in *; auto)).
+
+  Lemma lookup_remove_eq k l : lookup k (remove k l) = None.
+  Proof. induction l; simpler. Qed.
+
+  Lemma lookup_remove_neq k k' l : k <> k' -> lookup k (remove k' l) = lookup k l.
+  Proof. induction l; simpler. Qed.
+
+  Lemma lookup_none_remove k l : lookup k l = None -> remove k l = l.
+  Proof. induction l; simpler. f_equal; auto. Qed.
+
+  Lemma lookup_none_perm k l l' : Permutation l l' -> lookup k l = None -> lookup k l' = None.
+  Proof. induction 1; simpler. Qed.
+
+  Lemma distinct_remove k l : distinct l -> distinct (remove k l).
+  Proof. induction l; simpler; intuition. rewrite lookup_remove_neq; auto. Qed.
+
+  Lemma distinct_insert k (v:A.value_t k) l : distinct l -> distinct (insert v l).
+  Proof. induction l; simpler; intuition. rewrite lookup_remove_neq; auto. Qed.
+
+  Lemma distinct_perm l l' : Permutation l l' -> distinct l -> distinct l'.
+  Proof. Hint Resolve lookup_none_perm. induction 1; simpler; intuition (congruence||eauto). Qed.
+
+  Hint Resolve lookup_remove_eq distinct_remove distinct_perm Permutation_sym Permutation_refl.
+
+  Lemma lookup_dis_perm k l l' : Permutation l l' -> distinct l -> lookup k l = lookup k l'.
+  Proof. induction 1; simpler; intuition try congruence. clear H1 H2; congruence. rewrite H2. eauto. Qed.
+
+  Lemma remove_perm k l l' : Permutation l l' -> Permutation (remove k l) (remove k l').
+  Proof.  Hint Constructors Permutation. induction 1; simpler; eauto. Qed.
+  Hint Resolve remove_perm.
+
+  Lemma insert_perm k l l' (v:A.value_t k) : Permutation l l' -> Permutation (insert v l) (insert v l').
+  Proof. unfold insert; simpler. Qed.
+  Hint Resolve insert_perm.
+
+  Lemma remove_swap k k' l : remove k (remove k' l) = remove k' (remove k l).
+  Proof. induction l; simpler. Qed.
+  Hint Resolve remove_swap.
+
+  Lemma insert_swap k (v:A.value_t k) k' (v':A.value_t k') l : k <> k' -> 
+    Permutation (insert v (insert v' l)) (insert v' (insert v l)).
+  Proof. intros. Hint Constructors Permutation. unfold insert; simpler. rewrite remove_swap. auto. Qed.
+  Hint Resolve insert_swap.
 
 End AssocList.
 
@@ -95,7 +159,7 @@ Module FINITE_MAP_T(Assoc:ASSOCIATION)(AT:FINITE_MAP_AT with Module A:=Assoc).
   Definition insert :=
     forall (x:fmap_t)(k:A.key_t)(v:A.value_t k)(l:[alist_t]),
       STsep (l ~~ rep x l)
-        (fun (_:unit) => l ~~ rep x ((k,, v)::(remove k l))).
+        (fun (_:unit) => l ~~ rep x (insert v l)).
 
   (* lookup takes an fmap_t that represents some list l satisfying the predicate P, 
    * and a key k, and returns the value v associatied with k in l if any, while
@@ -112,77 +176,37 @@ Module FINITE_MAP_T(Assoc:ASSOCIATION)(AT:FINITE_MAP_AT with Module A:=Assoc).
         (fun (_:unit) => l ~~ rep x (remove k l)).
 
 (*
+  Fixpoint fold_pre (B:Type) (P0:B->hprop)
+    (P:forall k, A.value_t k->B->hprop)
+    (Q:forall k, A.value_t k->B->B->hprop) (b:B)
+    (l:alist_t) {struct l}:=
+  match l with 
+    | nil => P0 b
+    | (k,,v)::ls => P k v b * [forall b', Q k v b b' ==> fold_pre P0 P Q b' ls]
+  end.
+
+  Fixpoint fold_post (B:Type) (Q0:B->hprop)
+    (Q:forall k, A.value_t k->B->B->hprop) (b:B) (ans:B)
+    (l:alist_t) {struct l}:=
+  match l with 
+    | nil => Q0 b * [b=ans]
+    | (k,,v)::ls => Exists b' :@ B, Q k v b b' & fold_post Q0 Q b' ans ls
+  end.
+
   Definition hprop_forall T (p : T -> hprop) : hprop := fun h => forall v, p v h.
   Notation "'Forall' v :@ T , p" := (hprop_forall (fun v : T => p)) (at level 90, T at next level) : hprop_scope.
 
-  Definition hprop_himp (P Q : hprop) : hprop := fun h => P h -> Q h.
-  Notation "P ===> Q" := (hprop_himp P Q) (at level 85, T at next level) : hprop_scope.
-*)
-
-(*
-  (c:forall k v b l, insert destFM k v l),
-
-  (* fold *)
-  Fixpoint fold_pre (B C:Type) 
-    (P:alist_l->B->C->hprop)
-    (Q:alist_l->B->C->B->C->hprop) (b:B) (c:C)
-    (l:alist_t) {struct l}:=
-    P 
-  match l with 
-    | nil => P 
-    | (k,,v)::ls => P k v b c * [forall b' c', Q k v b c b' c' ==> fold_pre P Q b' c' ls]
-  end.
-
-
-  Fixpoint fold_pre (B C:Type) 
-    (P:forall k, A.value_t k->B->C->hprop)
-    (Q:forall k, A.value_t k->B->C->B->C->hprop) (b:B) (c:C)
-    (l:alist_t) {struct l}:=
-  match l with 
-    | nil => ??
-    | (k,,v)::ls => P k v b c * [forall b' c', Q k v b c b' c' ==> fold_pre P Q b' c' ls]
-  end.
-
-  Fixpoint fold_pre (B C:Type) 
-    (P:forall k, A.value_t k->B->C->hprop)
-    (Q:forall k, A.value_t k->B->C->B->C->hprop) (b:B) (c:C)
-    (l:alist_t) {struct l}:=
-  match l with 
-    | nil => ??
-    | (k,,v)::ls => P k v b c * [forall b' c', Q k v b c b' c' ==> fold_pre P Q b' c' ls]
-  end.
-
-  (* how to write this in seperation logic? *)
-  (* this actually uses the reverse list as fold_pre, but since we are
-     working upto permutation (see fold), this is ok *)
-
-  Fixpoint fold_post (B C:Type)
-    (Q:forall k, A.value_t k->B->C->B->C->hprop) (b:B) (c:C) (bans:B) (cans:C) 
-    (l:alist_t) {struct l}:=
-  match l with 
-    | nil => ?? * [b=bans] * [c=cans]
-    | (k,,v)::ls => Exists b' :@ B, Q k v ls b b' 
-  end.
-
-
-  Definition fold := forall (x:fmap_t)(B:Type) (P:forall k, A.value_t k->B->hprop)
-                                               (Q:forall k, A.value_t k->B->B->hprop) (b:B) 
+  Definition fold := forall (x:fmap_t)(B:Type) (P0:B->hprop) (P:forall k, A.value_t k->B->hprop) (Q0:B->hprop)
+                                               (Q:forall k, A.value_t k->B->B->hprop) (b:B)
                                                (c:forall k v b, STsep (P k v b) (Q k v b)) (l:[alist_t]),
-    STsep (l ~~ rep x l * Forall l' :@ {l':alist_t | Permutation l l'}, fold_pre B P Q (` l') b)
-    (fun (b':B) => (l ~~ rep x l * Exists l' :@ {l':alist_t | Permutation l l'}, fold_post B P Q (` l') b b')).
-
-
-  Fixpoint fold_post (B:Type) 
-    (Q:forall k, A.value_t k->B->B->hprop) (b:B) 
-    (l:alist_t) {struct l}:=
-  match l with 
-    | nil => ??
-    | (k,,v)::ls => P k v b & (Forall b' :@ B, Q k v b b' ===> fold_pre P Q b' ls)
-  end.
-  
+    STsep (l ~~ rep x l * Forall l' :@ {l':alist_t | Permutation l l'}, fold_pre P0 P Q b (proj1_sig l'))
+    (fun (b':B) => (l ~~ rep x l * Exists l' :@ {l':alist_t | Permutation l l'}, fold_post Q0 Q b b' (proj1_sig l'))).
 *)
+  Definition distinct := forall (x:fmap_t) (l:alist_t), rep x l ==> [distinct l] * ??.
 
-  Ltac unfm_t := unfold new, free, insert, lookup, remove.
+  Definition perm := forall (x:fmap_t) (l l':alist_t), Permutation l l' -> rep x l ==> rep x l'.
+
+  Ltac unfm_t := unfold new, free, insert, lookup, remove, distinct, perm.
 
 End FINITE_MAP_T.
 
@@ -192,7 +216,8 @@ End FINITE_MAP_T.
 Module Type FINITE_MAP.
 (* do we need A? *)
   Declare Module A  : ASSOCIATION.
-  Declare Module AT : FINITE_MAP_AT with Module A:=A.
+  Module AL := AssocList(A).
+  Declare Module AT : FINITE_MAP_AT with Module A:=A with Module AL := AL.
   Module T := FINITE_MAP_T(A)(AT).
 
   Export AT.
@@ -202,5 +227,107 @@ Module Type FINITE_MAP.
   Parameter insert : T.insert.
   Parameter remove : T.remove.
   Parameter lookup : T.lookup.
+(*  Parameter fold : T.fold. *)
+  Axiom distinct : T.distinct.
+  Axiom perm : T.perm.
 
 End FINITE_MAP.
+
+(*
+Module copier(FM:FINITE_MAP).
+Module AL := FM.AT.AL.
+Import AL.
+Import FM.
+
+Open Local Scope hprop_scope.
+Open Local Scope stsepi_scope.
+
+Fixpoint Tadd (sourceM destM:alist_t) {struct sourceM} :=
+  match sourceM with
+    | nil => destM
+    | (k,,v)::sourceM => AL.insert v (Tadd sourceM destM)
+  end.
+
+Lemma Tadd_perm1 l1 l1' l2 : Permutation l1 l1' -> AL.distinct l1 -> Permutation (Tadd l1 l2) (Tadd l1' l2).
+Proof. induction 1; simpler; intuition; try congruence. eapply perm_trans; eauto. Qed.
+
+Ltac simpl_inh := repeat 
+  match goal with
+    | [H:[_]%inhabited = [_]%inhabited |- _] => generalize (pack_injective H); clear H; intro H 
+    | [H1:?x = [?y1]%inhabited, H2:?x = [?y2]%inhabited |- _]
+      => match y1 with
+           | y2 => fail 1
+           | _ => rewrite H1 in H2
+         end
+  end.
+
+Lemma hprop_forall_conc T (P:T->hprop) Q : (forall x:T, Q ==> P x) -> Q ==> (T.hprop_forall P).
+Proof. firstorder. Qed.
+
+Ltac perm_simpl := 
+  match goal with
+  | [H:Permutation nil ?x |- _ ] => generalize (Permutation_nil H); clear H; intro H; subst x
+  | [H:Permutation ?x nil |- _ ] => generalize (Permutation_nil (Permutation_sym H)); clear H; intro H; subst x
+  | [H:Permutation (?a::?x1) ?x2 |- _ ] => 
+    match x2 with
+      | (_::_) => fail 1
+      | (_++_) => fail 1
+      | _ => destruct x2; [elim (Permutation_nil_cons (Permutation_sym H)) |]
+    end
+  | [H:Permutation ?x2 (?a::?x1) |- _ ] => 
+    match x2 with
+      | (_::_) => fail 1
+      | (_++_) => fail 1
+      | _ => destruct x2; [elim (Permutation_nil_cons H) |]
+    end
+end.
+
+Ltac simpler2 :=
+  repeat (progress ((repeat 
+    match goal with
+      | [H:[_]%inhabited = [_]%inhabited |- _] => generalize (pack_injective H); clear H; intro H 
+      | [H1:?x = [?y1]%inhabited, H2:?x = [?y2]%inhabited |- _]
+        => match y1 with
+             | y2 => fail 1
+             | _ => rewrite H1 in H2
+           end
+      | [|- context [match A.key_eq_dec ?k1 ?k2 with 
+                           | left _ => _ 
+                       | right _ => _ end]] =>
+      case_eq (A.key_eq_dec k1 k2) ; intros; try congruence ; try solve [assert False; intuition]; try subst
+        |[H: sigT _ |- _] => destruct H
+    end); simpl; auto)).
+
+Definition add (source ddest:fmap_t) (sourceM destM:[alist_t]) :
+  STsep (sourceM ~~ destM ~~ rep source sourceM * rep ddest destM)
+  (fun (_:unit) => sourceM ~~ destM ~~ rep source sourceM * rep ddest (Tadd sourceM destM)).
+intros.
+refine (zz <- (fold source _ _ _ _ destM (fun k v b => {{(insert ddest (k:=k) v b)}}
+                                         ;; {{Return (b ~~~ AL.insert v b)}}) sourceM)
+; {{Return tt}}); sep simpl_inh.
+assert (((fun (_:A.key_t) _ (x:[alist_t]) => (x ~~ rep ddest x)) k v [x]%inhabited) ==> rep ddest x); [idtac|eassumption].
+sep simpl_inh.
+assert (rep ddest (AL.insert v x0) ==> 
+   (fun _ _ l1 l2 => l2 ~~ rep ddest l2) k v [x0]%inhabited [AL.insert v x0]%inhabited); [idtac|eassumption].
+sep simpl_inh.
+apply hprop_forall_conc. destruct x1. simpl.
+revert x x0 p.
+induction x1; sep simpl_inh. 
+assert(rep ddest x ==> (fun x => x ~~ rep ddest x) [x]%inhabited); [sep simpl_inh|eassumption].
+destruct a.
+sep simpl_inh. repeat intro. destruct H. red. intuition. 
+sep auto.
+eapply IHx1. apply Permutation_refl.
+instantiate (1 := v). sep auto.
+instantiate (1 := v). sep auto.
+destruct v0. simpl.
+clear H2.
+revert x0 x2 p.
+induction x1; sep simpl_inh.
+
+perm_simpl. simpl. sep auto.
+assert((fun x => x ~~ rep ddest x) [x0]%inhabited ==> rep ddest x0); [sep simpl_inh|eassumption].
+perm_simpl. simpler. sep auto. sep auto. 
+pose (IHx1 x5 x2).
+
+*)
