examples/RefFiniteMap.v
@@ -12,9 +12,9 @@ Module RefAssocList(Assoc:ASSOCIATION) : FINITE_MAP with Module A := Assoc.
 
   Module AT <: FINITE_MAP_AT with Module A:=Assoc.
     Module A := Assoc.
-    Module AL := AssocList(Assoc).
+    Module AL := AssocList(Assoc). Import AL.
     Definition fmap_t := ptr.
-    Definition rep(x:fmap_t)(y:AL.alist_t) := (x --> y).
+    Definition rep(x:fmap_t)(y:alist_t) := Exists y' :@ alist_t, (x --> y') * [distinct y] * [Permutation y y'].
   End AT.
 
   Module T:=FINITE_MAP_T(Assoc)(AT).
@@ -25,7 +25,25 @@ Module RefAssocList(Assoc:ASSOCIATION) : FINITE_MAP with Module A := Assoc.
   Open Local Scope stsepi_scope.
 
   Ltac s := T.unfm_t; intros.
-  Ltac t := unfold rep; sep ltac:(subst; auto).
+
+Ltac sep' tac :=
+  let s := repeat progress (simpler; tac; try search_prem premer) in
+    let concer := apply himp_empty_conc
+      || apply himp_ex_conc_trivial
+        || (apply himp_ex_conc; econstructor)
+          || (eapply himp_unpack_conc; [eassumption || reflexivity |])
+            || (apply himp_inj_conc; [s; fail | idtac]) in
+              (intros; equater || specFinder; tac;
+                repeat match goal with
+                         | [ x : inhabited _ |- _ ] => dependent inversion x; clear x
+                       end;
+                intros; s;
+                  repeat ((
+                    search_prem ltac:(idtac;
+                      search_conc ltac:(apply himp_frame || (apply himp_frame_cell; trivial))) || search_conc concer);
+                  s);
+                  try finisher).
+  Ltac t := unfold rep; sep' ltac:(subst; eauto).
 
   Definition new : T.new. s;
     refine ({{New nil_al}})
@@ -37,8 +55,8 @@ Module RefAssocList(Assoc:ASSOCIATION) : FINITE_MAP with Module A := Assoc.
 
   Definition lookup : T.lookup. s;
     refine (z <- ! x ; 
-            {{Return (lookup k z)}})
-  ; t. Defined.
+            {{Return (lookup k z)}}) ; t. rewrite (lookup_dis_perm k H1); t.
+  Defined.
 
   Definition insert :  T.insert. s;
     refine (z <- ! x ;
@@ -49,5 +67,8 @@ Module RefAssocList(Assoc:ASSOCIATION) : FINITE_MAP with Module A := Assoc.
     refine (z <- ! x ;
             {{x ::= (remove k z)}})
   ; t. Defined.
+
+  Lemma perm : T.perm. s; t. Qed.
+  Lemma distinct : T.distinct. s; t. Qed.
 
 End RefAssocList.
